theories/interpreter.v
@@ -159,7 +159,14 @@ Definition run_one_step (call : run_stepE ~> itree (run_stepE +' eff))
 
   | AI_basic BI_handleadd =>
       if ves is VAL_handle h :: VAL_int32 c :: ves' then
-        (ret (s, f, RS_normal (vs_to_es (VAL_handle (handle_add h (Wasm_int.Z_of_sint i32m c)) :: ves'))))
+        expect (handle_add h (Wasm_int.Z_of_sint i32m c))
+          (fun v => (ret (s, f, RS_normal (vs_to_es (VAL_handle v :: ves')))))
+          (ret (s, f, RS_normal ((vs_to_es ves') ++ [::AI_trap])))
+      else ret (s, f, crash_error)
+
+  | AI_basic BI_getoffset =>
+      if ves is VAL_handle h :: ves' then
+        ret (s, f, RS_normal (vs_to_es (VAL_int32 (Wasm_int.int_of_Z i32m (Z.of_N (offset h))) :: ves' )))
       else ret (s, f, crash_error)
           
   (** testops **)
@@ -350,7 +357,7 @@ Definition run_one_step (call : run_stepE ~> itree (run_stepE +' eff))
                (fun j' =>
                   if List.nth_error s.(s_segs) j is Some seg_s_j then
                     if List.nth_error s.(s_alls) j' is Some all_s_j' then *)
-                      if h.(valid) && (Z.leb 0 h.(offset)) && (N.leb (Z.to_N h.(offset) + N.of_nat (t_length T_handle)) h.(bound)) && isAllocb h.(id) s.(s_alls) && (N.eqb (N.modulo (handle_addr h) (N.of_nat (t_length T_handle))) (N.of_nat 0))
+                      if h.(valid) && (N.leb (h.(offset) + N.of_nat (t_length T_handle)) h.(bound)) && isAllocb h.(id) s.(s_alls) && (N.eqb (N.modulo (handle_addr h) (N.of_nat (t_length T_handle))) (N.of_nat 0))
                       then expect
                              (segload s.(s_segs) h (t_length T_handle))
                              (fun bs =>
@@ -375,7 +382,7 @@ Definition run_one_step (call : run_stepE ~> itree (run_stepE +' eff))
                (fun j' =>
                   if List.nth_error s.(s_segs) j is Some seg_s_j then
                     if List.nth_error s.(s_alls) j' is Some all_s_j' then *)
-                      if h.(valid) && (Z.leb 0 h.(offset)) && (N.leb (Z.to_N h.(offset) + N.of_nat (t_length T_handle)) h.(bound)) && isAllocb h.(id) s.(s_alls) && (N.eqb (N.modulo (handle_addr h) (N.of_nat (t_length T_handle))) (N.of_nat 0))
+                      if h.(valid) && (N.leb (h.(offset) + N.of_nat (t_length T_handle)) h.(bound)) && isAllocb h.(id) s.(s_alls) && (N.eqb (N.modulo (handle_addr h) (N.of_nat (t_length T_handle))) (N.of_nat 0))
                       then expect
                              (segstore s.(s_segs) h (List.map (fun x => (x, Handle)) (bits v)) (t_length T_handle))
                              (fun seg' =>
@@ -401,7 +408,7 @@ Definition run_one_step (call : run_stepE ~> itree (run_stepE +' eff))
                (fun j' =>
                   if List.nth_error s.(s_segs) j is Some seg_s_j then
                     if List.nth_error s.(s_alls) j' is Some all_s_j' then *)
-                      if h.(valid) && (Z.leb 0 h.(offset)) && (N.leb (Z.to_N h.(offset) + N.of_nat (t_length t)) h.(bound)) && isAllocb h.(id) s.(s_alls)
+                      if h.(valid) && (N.leb (h.(offset) + N.of_nat (t_length t)) h.(bound)) && isAllocb h.(id) s.(s_alls)
                       then expect
                              (segload s.(s_segs) h (t_length t))
                              (fun bs => ret (s, f, RS_normal (vs_to_es (wasm_deserialise (List.map fst bs) t :: ves'))))
@@ -423,7 +430,7 @@ Definition run_one_step (call : run_stepE ~> itree (run_stepE +' eff))
                (fun j' =>
                   if List.nth_error s.(s_segs) j is Some seg_s_j then
                     if List.nth_error s.(s_alls) j' is Some all_s_j' then *)
-                      if h.(valid) && (Z.leb 0 h.(offset)) && (N.leb (Z.to_N h.(offset) + N.of_nat (t_length t)) h.(bound)) && isAllocb h.(id) s.(s_alls)
+                      if h.(valid) && (N.leb (h.(offset) + N.of_nat (t_length t)) h.(bound)) && isAllocb h.(id) s.(s_alls)
                       then expect
                              (segstore s.(s_segs) h (List.map (fun x => (x, Numeric)) (bits v)) (t_length t))
                              (fun seg' =>
@@ -531,7 +538,7 @@ Definition run_one_step (call : run_stepE ~> itree (run_stepE +' eff))
                (fun j' =>
                   if List.nth_error s.(s_segs) j is Some s_seg_s_j then
                     if List.nth_error s.(s_alls) j' is Some s_all_s_j' then *)
-                      if h.(valid) && (h.(offset) == Z.zero)%Z then
+                      if h.(valid) && (h.(offset) == N.zero)%N then
                         expect
                           (find_and_remove h.(id) s.(s_alls).(allocated))
                           (fun '(l, a, n) =>
